working on the core of RTac.

theories/RTac/Assumption.v
@@ -1,3 +1,5 @@
+Require Import ExtLib.Data.Sum.
+Require Import ExtLib.Data.HList.
 Require Import ExtLib.Tactics.
 Require Import MirrorCore.EnvI.
 Require Import MirrorCore.SymI.
@@ -25,32 +27,131 @@ Section parameterized.
   Context {SubstUpdate_subst : SubstUpdate subst expr}.
   Context {SubstUpdateOk_subst : @SubstUpdateOk _ _ _ _ Expr_expr Subst_subst _ _}.
 
-  Variable (check : Ctx typ expr -> expr -> expr -> subst -> option subst).
+  Section findHyp.
+    Variable check : expr -> subst -> option subst.
 
-  Fixpoint findHyp s (ctx : Ctx typ expr) (g : expr) {struct ctx}
-  : option subst :=
-    match ctx with
-      | CTop => None
-      | CAll ctx' _ => findHyp s ctx' g
-      | CEx  ctx' _ => findHyp s ctx' g
-      | CHyp ctx' h => match check ctx' g h s with
-                         | None => findHyp s ctx' g
-                         | Some e => Some e
-                       end
-    end.
+    Fixpoint findHyp (ctx : Ctx typ expr) (s : subst) {struct ctx}
+    : option subst :=
+      match ctx with
+        | CTop => None
+        | CAll ctx' _ => findHyp ctx' s
+        | CEx  ctx' _ => findHyp ctx' s
+        | CHyp ctx' h => match check h s with
+                           | None => findHyp ctx' s
+                           | Some e => Some e
+                         end
+      end.
+  End findHyp.
+
+  Variable check : Ctx typ expr -> expr -> expr -> subst -> option subst.
 
   Definition ASSUMPTION : rtac typ expr subst :=
     fun ctx s gl =>
-      match findHyp s ctx gl with
+      match findHyp (check ctx gl) ctx s with
         | None => Fail
         | Some s' =>
           Solved s'
       end.
+(*
+  Definition exprD'_ctx (ctx : Ctx typ expr) (e : expr) (t : typ)
+  : option (OpenT (getUVars ctx) (getVars ctx) (typD t)) :=
+    exprD' (getUVars ctx) (getVars ctx) e t.
+*)
+  Hypothesis checkOk
+  : forall ctx e1 e2 s s',
+      check ctx e1 e2 s = Some s' ->
+      WellFormed_subst s ->
+      let tus := getUVars ctx nil in
+      let tvs := getVars ctx nil in
+      WellFormed_subst s' /\
+      forall v1 v2 sD,
+        exprD' tus tvs e1 (@typ0 _ _ Prop _) = Some v1 ->
+        exprD' tus tvs e1 (@typ0 _ _ Prop _) = Some v2 ->
+        substD tus tvs s = Some sD ->
+        exists sD',
+             substD tus tvs s' = Some sD'
+          /\ forall us vs,
+               sD' us vs ->
+               sD us vs /\
+               v1 us vs = v2 us vs.
 
-  (** check soundness **)
+  Theorem rev_app_distr_trans
+  : forall (A : Type) (x y : list A), rev (x ++ y) = rev y ++ rev x.
+  Proof. clear.
+         induction x; simpl; intros.
+         - symmetry. apply app_nil_r_trans.
+         - rewrite IHx. apply app_ass_trans.
+  Defined.
 
-End parameterized.
+  (** TODO: This is cubic! **)
+  Theorem rev_involutive_trans (A : Type)
+  : forall (l : list A), rev (rev l) = l.
+  Proof. clear.
+         induction l; simpl; auto.
+         rewrite rev_app_distr. rewrite IHl. reflexivity.
+  Defined.
+
+  Definition hlist_unrev {T} {F : T -> Type} {ls} (h : hlist F (rev ls))
+  : hlist F ls :=
+    match rev_involutive_trans ls in _ = t return hlist F t with
+      | eq_refl => hlist_rev h
+    end.
 
 (*
+  Lemma findHypOk
+  : forall ctx tus tvs g s s',
+      findHyp (check ctx (** TODO: This isn't right **) g) ctx s = Some s' ->
+      WellFormed_subst s ->
+      WellFormed_subst s' /\
+      let tus' := tus ++ getUVars ctx nil in
+      let tvs' := tvs ++ getVars ctx nil in
+      match propD  tus' tvs' g
+          , substD tus' tvs' s
+          , substD tus' tvs' s'
+      with
+        | Some gD , Some sD , Some sD' =>
+          ctxD' ctx (fun (us : hlist _ (rev tus')) (vs : hlist _ (rev tvs')) =>
+                       let us := hlist_unrev us in
+                       let vs := hlist_unrev vs in
+                       sD' us vs ->
+                       sD us vs /\ gD us vs)
+        | None , _ , _
+        | _ , None , _ => True
+        | Some _ , Some _ , None => False
+      end.
+  Proof.
+    induction ctx; simpl; intros; try congruence.
+    { specialize (IHctx tus (tvs ++ t :: nil) _ _ _ H H0).
+      forward_reason; split; eauto.
+      forward.
+      subst.
+      eapply substD_weakenV with (tvs' := t :: nil) in H4.
+      eapply exprD'_typ0_weakenV with (tvs' := t :: nil) in H3.
+      forward_reason.
+      rewrite H4 in H2.
+      change_rewrite H3 in H2.
+      forwardy.
+      rewrite 
+ }
+    { specialize (IHctx (tus ++ t :: nil) tvs _ _ _ H H0).
+      forward_reason; split; eauto.
+      forward.
+      subst. eapply H4. }
+    { consider (check ctx g e s); intros.
+      { clear IHctx. inv_all; subst.
+        eapply checkOk in H; clear checkOk; eauto.
+        forward_reason; split; eauto.
+        forward.
+        destruct o0; inv_all; subst.
+        { admit. }
+        { 
 
+
+  Theorem ASSUMPTION_sound : rtac_sound nil nil ASSUMPTION.
+  Proof.
+    unfold ASSUMPTION, rtac_sound.
+    intros. subst.
+    consider (findHyp s ctx g); auto.
+    intros.
 *)
+End parameterized.
